src/michocoq/syntax.v
@@ -280,8 +280,11 @@ Inductive signature_constant : Set := Mk_sig : str -> signature_constant.
 Inductive key_constant : Set := Mk_key : str -> key_constant.
 Inductive key_hash_constant : Set := Mk_key_hash : str -> key_hash_constant.
 Inductive tez_constant : Set := Mk_tez : str -> tez_constant.
-Inductive contract_constant : Set := Mk_contract : str -> contract_constant.
-Inductive address_constant : Set := Mk_address : str -> address_constant.
+Inductive smart_contract_address_constant : Set :=
+| Mk_smart_contract_address : str -> smart_contract_address_constant.
+Inductive address_constant : Set :=
+| Implicit : key_hash_constant -> address_constant
+| Originated : smart_contract_address_constant -> address_constant.
 Inductive operation_constant : Set := Mk_operation : str -> operation_constant.
 Inductive mutez_constant : Set := Mk_mutez : tez.mutez -> mutez_constant.
 Inductive chain_id_constant : Set := Mk_chain_id : str -> chain_id_constant.
